{
 "cells": [
  {
   "cell_type": "markdown",
   "metadata": {},
   "source": [
    "# Convexity\n",
    "\n",
    "[Back to index](https://shotahorii.github.io/math-for-ds/)\n",
    "\n",
    "---\n",
    "\n",
    "## Table of contents\n",
    "1. **Convex set**  \n",
    "1.1. Definition of a convex set  \n",
    "1.2. Examples of convex set  \n",
    "1.3. Basic property  \n",
    "2. **Convex function**  \n",
    "2.1. Definition of a convex function  \n",
    "2.2. First-order convexity condition  \n",
    "2.3. Second-order convexity condition\n",
    "\n",
    "---"
   ]
  },
  {
   "cell_type": "markdown",
   "metadata": {},
   "source": [
    "## 1. Convex set\n",
    "\n",
    "### 1.1. Definition of a convex set\n",
    "\n",
    "A set $A \\subseteq \\mathbb{R}^d$ is a **convex set** when $t{\\bf x}^{(1)} + (1-t){\\bf x}^{(2)} \\in A$ is always true for any pair of ${\\bf x}^{(1)} \\in A$ and ${\\bf x}^{(2)} \\in A$, with any $t \\in [0,1]$.\n",
    "\n",
    "---\n",
    "\n",
    "\n",
    "### 1.2. Examples of convex set\n",
    "\n",
    "**Example 1**\n",
    "\n",
    "$A = \\{{\\bf x}|{\\bf m}\\cdot{\\bf x}+b = 0, {\\bf x}\\in \\mathbb{R}^d\\}$\n",
    "\n",
    "**Proof**\n",
    "\n",
    "Let: ${\\bf x}^{(1)},{\\bf x}^{(2)} \\in A $\n",
    "\n",
    "${\\bf x}^{(1)},{\\bf x}^{(2)} \\in A \\Longrightarrow {\\bf m}\\cdot{\\bf x}^{(1)} = -b, \\,\\,\\, {\\bf m}\\cdot{\\bf x}^{(2)} = -b$\n",
    "\n",
    "Let: $t \\in [0,1]$\n",
    "\n",
    "${\\bf m}\\cdot\\{t{\\bf x}^{(1)} + (1-t){\\bf x}^{(2)}\\} + b$\n",
    "\n",
    "$= t{\\bf m}\\cdot{\\bf x}^{(1)} + (1-t){\\bf m}\\cdot{\\bf x}^{(2)} + b$\n",
    "\n",
    "$= t(-b)+(1-t)(-b)+b = 0$\n",
    "\n",
    "**Example 2**\n",
    "\n",
    "$A = \\{{\\bf x}|{\\bf m}\\cdot{\\bf x}+b \\ge 0, {\\bf x}\\in \\mathbb{R}^d\\}$\n",
    "\n",
    "**Proof**\n",
    "\n",
    "Let: ${\\bf x}^{(1)},{\\bf x}^{(2)} \\in A $\n",
    "\n",
    "${\\bf x}^{(1)},{\\bf x}^{(2)} \\in A \\Longrightarrow {\\bf m}\\cdot{\\bf x}^{(1)} \\ge -b, \\,\\,\\, {\\bf m}\\cdot{\\bf x}^{(2)} \\ge -b$\n",
    "\n",
    "Let: $t \\in [0,1]$\n",
    "\n",
    "$t \\in [0,1] \\Longrightarrow t \\ge 0, \\,\\,\\, (1-t) \\ge 0$\n",
    "\n",
    "${\\bf m}\\cdot\\{t{\\bf x}^{(1)} + (1-t){\\bf x}^{(2)}\\} + b$\n",
    "\n",
    "$= t{\\bf m}\\cdot{\\bf x}^{(1)} + (1-t){\\bf m}\\cdot{\\bf x}^{(2)} + b$\n",
    "\n",
    "$\\ge t(-b)+(1-t)(-b)+b = 0$\n",
    "\n",
    "---\n",
    "\n",
    "### 1.3. Basic property\n",
    "\n",
    "When each of $A$ and $B$ is a convex set, $A \\cap B$ is a convex set.\n",
    "\n",
    "**Proof**\n",
    "\n",
    "Let: ${\\bf x}^{(1)},{\\bf x}^{(2)} \\in A\\cap B$\n",
    "\n",
    "${\\bf x}^{(1)},{\\bf x}^{(2)} \\in A\\cap B \\Longrightarrow {\\bf x}^{(1)},{\\bf x}^{(2)} \\in A \\Longrightarrow t{\\bf x}^{(1)} + (1-t){\\bf x}^{(2)} \\in A$\n",
    "\n",
    "${\\bf x}^{(1)},{\\bf x}^{(2)} \\in A\\cap B \\Longrightarrow {\\bf x}^{(1)},{\\bf x}^{(2)} \\in B \\Longrightarrow t{\\bf x}^{(1)} + (1-t){\\bf x}^{(2)} \\in B$\n",
    "\n",
    "Hence, \n",
    "\n",
    "$t{\\bf x}^{(1)} + (1-t){\\bf x}^{(2)} \\in A\\cap B$\n",
    "\n",
    "**Note**\n",
    "\n",
    "$A \\cup B$ is not always a convex function even when each of $A$ and $B$ is a convex set.\n",
    "\n",
    "---"
   ]
  },
  {
   "cell_type": "markdown",
   "metadata": {},
   "source": [
    "## 2. Convex function\n",
    "\n",
    "### 2.1. Definition of a convex function\n",
    "\n",
    "A function $f({\\bf x})$ is a **convex function** when $f(t{\\bf x}^{(1)} + (1-t){\\bf x}^{(2)}) \\le tf({\\bf x}^{(1)})+(1-t)f({\\bf x}^{(2)})$ is always true for any pair of ${\\bf x}^{(1)},{\\bf x}^{(2)} \\in \\mathbb{R}^d$, with any $t \\in [0,1]$.\n",
    "\n",
    "#### Another definition using epigraph\n",
    "\n",
    "Given a function $f$, a set defined as below is called an epigraph.\n",
    "\n",
    "$epi\\,f = \\{({\\bf x},y) \\in \\mathbb{R}^d \\times \\mathbb{R} | y \\ge f({\\bf x})\\}$\n",
    "\n",
    "A function $f({\\bf x})$ is a convex function if $epi\\,f$ is a convex set.\n",
    "\n",
    "---\n",
    "\n",
    "### 2.2. First-order convexity condition\n",
    "\n",
    "Let: $\\nabla f({\\bf u})= (\\frac{\\partial f({\\bf x})}{\\partial x_1},\\frac{\\partial f({\\bf x})}{\\partial x_2},...,\\frac{\\partial f({\\bf x})}{\\partial x_d})^T |_{{\\bf x}={\\bf u}} \\,\\,\\, , {\\bf u} \\in \\mathbb{R}^d$\n",
    "\n",
    "$f({\\bf x})$ is a convex function $\\Longleftrightarrow f({\\bf v}) \\ge f({\\bf u}) + \\nabla f({\\bf u})\\cdot({\\bf v}-{\\bf u}) \\,\\,\\,\\,\\, ({\\bf u}, {\\bf v} \\in \\mathbb{R}^d)$\n",
    "\n",
    "#### Proof  (when d=1)\n",
    "\n",
    "Let: $f(x)$ be a convex function, $u,v \\in \\mathbb{R}$\n",
    "\n",
    "$f(tv + (1-t)u) \\le tf(v)+(1-t)f(u)$\n",
    "\n",
    "$\\Longrightarrow f(u + t(v-u)) \\le f(u) + t(f(v)-f(u))$\n",
    "\n",
    "$\\Longrightarrow \\frac{f(u + t(v-u)) - f(u)}{t} \\le f(v)-f(u)$\n",
    "\n",
    "$\\Longrightarrow \\frac{f(u + t(v-u)) - f(u)}{t(v-u)}(v-u) \\le f(v)-f(u)$\n",
    "\n",
    "As this inequality is true for any $t \\in [0,1]$, let $t \\to 0$\n",
    "\n",
    "Let: $h = t(v-u)$ then, $t \\to 0 \\Rightarrow h \\to 0$\n",
    "\n",
    "$\\Longrightarrow \\lim\\limits_{h \\to 0} \\frac{f(u + h) - f(u)}{h}(v-u) \\le f(v)-f(u)$\n",
    "\n",
    "$\\Longrightarrow f'(u)(v-u) \\le f(v)-f(u)$\n",
    "\n",
    "$\\Longrightarrow f(v) \\ge f(u) + f'(u)(v-u)$\n",
    "\n",
    "#### Proof (in general - not only when d=1)\n",
    "\n",
    "Let: $f({\\bf x})$ be a convex function, ${\\bf u}, {\\bf v} \\in \\mathbb{R}^d$\n",
    "\n",
    "$tf({\\bf v})+(1-t)f({\\bf u}) \\ge f(t{\\bf v} + (1-t){\\bf u}) = f({\\bf u} + t({\\bf v}-{\\bf u}))$\n",
    "\n",
    "Note: With Taylor series, $f({\\bf u} + t({\\bf v}-{\\bf u})) = f({\\bf u}) + \\nabla f({\\bf u})\\cdot\\{t({\\bf v}-{\\bf u})\\} + o(t||{\\bf v}-{\\bf u}||) $\n",
    "\n",
    "$\\Longrightarrow tf({\\bf v})+(1-t)f({\\bf u}) \\ge f({\\bf u}) + \\nabla f({\\bf u})\\cdot\\{t({\\bf v}-{\\bf u})\\} + o(t||{\\bf v}-{\\bf u}||)$\n",
    "\n",
    "$\\Longrightarrow tf({\\bf v}) \\ge tf({\\bf u}) + \\nabla f({\\bf u})\\cdot\\{t({\\bf v}-{\\bf u})\\} + o(t||{\\bf v}-{\\bf u}||)$\n",
    "\n",
    "$\\Longrightarrow f({\\bf v}) \\ge f({\\bf u}) + \\nabla f({\\bf u})\\cdot({\\bf v}-{\\bf u}) + \\frac{o(t||{\\bf v}-{\\bf u}||)}{t}$\n",
    "\n",
    "Let: $t \\to 0$\n",
    "\n",
    "Note: $\\lim\\limits_{t \\to 0}\\frac{o(t||{\\bf v}-{\\bf u}||)}{t} = 0$\n",
    "\n",
    "$\\Longrightarrow f({\\bf v}) \\ge f({\\bf u}) + \\nabla f({\\bf u})\\cdot({\\bf v}-{\\bf u})$\n",
    "\n",
    "---"
   ]
  },
  {
   "cell_type": "markdown",
   "metadata": {},
   "source": [
    "### 2.3. Second-order convexity condition\n",
    "\n",
    "Let: the Hessian $H_{\\bf x} = \\nabla^2f({\\bf x})$ as $\\nabla^2f({\\bf x})_{ij} = \\frac{\\partial^2f({\\bf x})}{\\partial x_i \\partial x_j}, \\,\\,\\,\\,\\, i,j = 1,2,...,d$\n",
    "\n",
    "$f({\\bf x})$ is a convex function $\\Longleftrightarrow H_{\\bf x}$ is positive semi-definite\n",
    "\n",
    "In other words,\n",
    "\n",
    "$f({\\bf x})$ is a convex function $\\Longleftrightarrow {\\bf u}^T\\nabla^2f({\\bf x}){\\bf u}$ for any ${\\bf x}, {\\bf u} \\in \\mathbb{R}^d$\n",
    "\n",
    "#### Proof (when d=1)\n",
    "\n",
    "Let: $f(x)$ be a convex function, $u,v \\in \\mathbb{R}$\n",
    "\n",
    "$f(v) \\ge f(u) + f'(u)(v-u)$\n",
    "\n",
    "Let: $v = u + \\delta u$\n",
    "\n",
    "$f(u + \\delta u) \\ge f(u) + f'(u)\\delta u$\n",
    "\n",
    "Note: with Taylor series, $f(u + \\delta u) = f(u) + f'(u)\\delta u + \\frac{f''(u)}{2}(\\delta u)^2 + o((\\delta u)^2)$\n",
    "\n",
    "$\\Longrightarrow f(u) + f'(u)\\delta u + \\frac{f''(u)}{2}(\\delta u)^2 + o((\\delta u)^2) \\ge f(u) + f'(u)\\delta u$\n",
    "\n",
    "$\\Longrightarrow \\frac{f''(u)}{2}(\\delta u)^2 + o((\\delta u)^2) \\ge 0$\n",
    "\n",
    "$\\Longrightarrow \\frac{f''(u)}{2} + \\frac{o((\\delta u)^2)}{(\\delta u)^2} \\ge 0$\n",
    "\n",
    "Let: $t \\to 0$\n",
    "\n",
    "Note: $\\lim\\limits_{\\delta u \\to 0}\\frac{o((\\delta u)^2)}{(\\delta u)^2} = 0$\n",
    "\n",
    "$\\Longrightarrow f''(u) \\ge 0$\n",
    "\n",
    "#### Proof (in general - not only when d=1)\n",
    "\n",
    "Let: $f({\\bf x})$ be a convex function, ${\\bf u},{\\bf d} \\in \\mathbb{R}^d, \\lambda > 0$\n",
    "\n",
    "$f({\\bf u} + \\lambda {\\bf d}) \\ge f({\\bf u}) + \\lambda \\nabla f({\\bf u})^T{\\bf d}$\n",
    "\n",
    "Note: with Taylor series, $f({\\bf u} + \\lambda {\\bf d}) = f({\\bf u}) + \\lambda \\nabla f({\\bf u})^T{\\bf d} + \\frac{\\lambda^2}{2} {\\bf d}^T \\nabla^2 f({\\bf u}){\\bf d} + o(\\lambda^2)$\n",
    "\n",
    "$\\Longrightarrow f({\\bf u}) + \\lambda \\nabla f({\\bf u})^T{\\bf d} + \\frac{\\lambda^2}{2} {\\bf d}^T \\nabla^2 f({\\bf u}){\\bf d} + o(\\lambda^2) \\ge f({\\bf u}) + \\lambda \\nabla f({\\bf u})^T{\\bf d}$\n",
    "\n",
    "$\\Longrightarrow \\frac{\\lambda^2}{2} {\\bf d}^T \\nabla^2 f({\\bf u}){\\bf d} + o(\\lambda^2) \\ge 0$\n",
    "\n",
    "$\\Longrightarrow \\frac{1}{2} {\\bf d}^T \\nabla^2 f({\\bf u}){\\bf d} + \\frac{o(\\lambda^2)}{\\lambda^2} \\ge 0$\n",
    "\n",
    "Let: $\\lambda \\to 0$\n",
    "\n",
    "Note: $\\lim\\limits_{\\lambda \\to 0}\\frac{o(\\lambda^2)}{\\lambda^2} = 0$\n",
    "\n",
    "$\\Longrightarrow {\\bf d}^T \\nabla^2 f({\\bf u}){\\bf d} \\ge 0$"
   ]
  }
 ],
 "metadata": {
  "kernelspec": {
   "display_name": "Python 3",
   "language": "python",
   "name": "python3"
  },
  "language_info": {
   "codemirror_mode": {
    "name": "ipython",
    "version": 3
   },
   "file_extension": ".py",
   "mimetype": "text/x-python",
   "name": "python",
   "nbconvert_exporter": "python",
   "pygments_lexer": "ipython3",
   "version": "3.5.6"
  }
 },
 "nbformat": 4,
 "nbformat_minor": 2
}
