{
 "cells": [
  {
   "cell_type": "markdown",
   "metadata": {},
   "source": [
    "# Binomial and Multinomial Theorem\n",
    "\n",
    "[Back to index](https://shotahorii.github.io/math-for-ds/)\n",
    "\n",
    "---\n",
    "\n",
    "## Table of contents\n",
    "1. Binomial Theorem\n",
    "2. Multinomial Theorem\n",
    "\n",
    "---\n",
    "\n"
   ]
  },
  {
   "cell_type": "markdown",
   "metadata": {},
   "source": [
    "## 1. Binomial Theorem\n",
    "\n",
    "$ (x+y)^N=\\sum^N_{m=0} \\left(\\begin{array}{c}N\\\\m\\\\\\end{array}\\right)x^{N-m} y^m = \\sum^N_{m=0} \\frac{N!}{(N-m)!m!}x^{N-m} y^m$\n",
    "\n",
    "$ where\\,\\,\\,\\, N,m \\in \\mathbb{N}_0 $\n",
    "\n",
    "See [Binomial Coefficient](https://github.com/shotahorii/math-for-ds/blob/master/content/others/binomial_coefficient.ipynb)\n",
    "\n",
    "#### Proof by induction\n",
    "\n",
    "When $N=1$\n",
    "\n",
    "$ x+y = \\sum^1_{m=0} \\frac{1!}{(1-m)!m!}x^{1-m} y^m = \\frac{1!}{1!0!}x^1y^0 + \\frac{1!}{0!1!}x^0 y^1 = x + y$\n",
    "\n",
    "Proof that the theorem is true when $N=k+1$ if the theorem is true when $N=k$.\n",
    "\n",
    "$(x+y)^k=\\sum^k_{m=0} \\left(\\begin{array}{c}k\\\\m\\\\\\end{array}\\right)x^{k-m} y^m$\n",
    "\n",
    "$\\Longrightarrow (x+y)^{k+1}=(x+y) \\sum^{k}_{m=0} \\left(\\begin{array}{c}k\\\\m\\\\\\end{array}\\right)x^{k-m} y^m$\n",
    "\n",
    "$= \\sum^{k}_{m=0} \\left(\\begin{array}{c}k\\\\m\\\\\\end{array}\\right)x^{k-m+1} y^m + \\sum^{k}_{m=0} \\left(\\begin{array}{c}k\\\\m\\\\\\end{array}\\right)x^{k-m} y^{m+1}$\n",
    "\n",
    "$= x^{k+1}+\\sum^{k}_{m=1} \\left(\\begin{array}{c}k\\\\m\\\\\\end{array}\\right)x^{k-m+1} y^m + \\sum^{k-1}_{m=0} \\left(\\begin{array}{c}k\\\\m\\\\\\end{array}\\right)x^{k-m} y^{m+1} + y^{k+1}$\n",
    "\n",
    "Let: $m' = m+1$\n",
    "\n",
    "$= x^{k+1}+\\sum^{k}_{m=1} \\left(\\begin{array}{c}k\\\\m\\\\\\end{array}\\right)x^{k-m+1} y^m + \\sum^{k}_{m'=1} \\left(\\begin{array}{c}k\\\\m'-1\\\\\\end{array}\\right)x^{k-m'+1} y^{m'} + y^{k+1}$\n",
    "\n",
    "$= x^{k+1}+\\sum^{k}_{m=1} \\{ \\left(\\begin{array}{c}k\\\\m\\\\\\end{array}\\right) + \\left(\\begin{array}{c}k\\\\m-1\\\\\\end{array}\\right) \\} x^{k-m+1} y^m + y^{k+1}$\n",
    "\n",
    "$= x^{k+1}+\\sum^{k}_{m=1} \\left(\\begin{array}{c}k+1\\\\m\\\\\\end{array}\\right) x^{k-m+1} y^m + y^{k+1}$\n",
    "\n",
    "$= \\sum^{k+1}_{m=0} \\left(\\begin{array}{c}k+1\\\\m\\\\\\end{array}\\right) x^{k+1-m} y^m$\n",
    "\n",
    "---"
   ]
  },
  {
   "cell_type": "markdown",
   "metadata": {},
   "source": [
    "## 2. Multinomial Theorem\n",
    "\n",
    "The coefficient of $x_1^{m_1}x_2^{m_2}...x_K^{m_K}$ in the expansion of $(x_1 + x_2 + ... + x_K)^N$ is $\\frac{N!}{m_1!m_2!...m_K!}$ \n",
    "\n",
    "Where $N, m_k \\in \\mathbb{N}_0 , \\,\\,\\, \\sum_{k=1}^K m_k = N$\n",
    "\n",
    "In other words,\n",
    "\n",
    "$(x_1 + x_2 + ... + x_K)^N = \\sum_{\\sum m_k = N} \\frac{N!}{m_1!m_2!...m_K!} \\prod_{k=1}^K x_k^{m_k}$\n",
    "\n",
    "#### Proof by induction\n",
    "\n",
    "When $K=1$\n",
    "\n",
    "$x_1^N = \\sum_{m_1 = N} \\frac{N!}{m_1!} \\prod_{k=1}^1 x_1^{m_1} = x_1^N$\n",
    "\n",
    "Proof that the theorem is true when $K=r+1$ if the theorem is true when $K=r$.\n",
    "\n",
    "$(x_1 + x_2 + ... + x_r + x_{r+1})^N = ((x_1 + x_2 + ... + x_r) + x_{r+1})^N$\n",
    "\n",
    "Applying binomial theorem,\n",
    "\n",
    "$= \\sum_{i=0}^N \\frac{N!}{i!(N-i)!} x_{r+1}^i(x_1 + x_2 + ... + x_r)^{N-i}$\n",
    "\n",
    "Note: As assuming the theorem is true when $K=r$, $(x_1 + x_2 + ... + x_r)^{N-i} = \\sum_{m_1+m_2+...+m_r = N-i} \\frac{(N-i)!}{m_1!m_2!...m_r!} \\prod_{k=1}^r x_k^{m_k}$\n",
    "\n",
    "$= \\sum_{i=0}^N \\left( \\frac{N!}{i!(N-i)!} x_{r+1}^i\\sum_{m_1+m_2+...+m_r = N-i} \\frac{(N-i)!}{m_1!m_2!...m_r!} \\prod_{k=1}^r x_k^{m_k} \\right)$\n",
    "\n",
    "Renaming index variable $i$ to $m_{r+1}$\n",
    "\n",
    "$= \\sum_{m_{r+1}=0}^N \\left( \\frac{N!}{m_{r+1}!(N-m_{r+1})!} x_{r+1}^{m_{r+1}}\\sum_{m_1+m_2+...+m_r = N-m_{r+1}} \\frac{(N-m_{r+1})!}{m_1!m_2!...m_r!} \\prod_{k=1}^r x_k^{m_k} \\right)$\n",
    "\n",
    "$= \\sum_{m_{r+1}=0}^N \\left(\\sum_{m_1+m_2+...+m_r = N-m_{r+1}} \\frac{N!}{m_{r+1}!(N-m_{r+1})!}\\frac{(N-m_{r+1})!}{m_1!m_2!...m_r!} \\prod_{k=1}^{r+1} x_k^{m_k} \\right)$\n",
    "\n",
    "$= \\sum_{m_{r+1}=0}^N \\left(\\sum_{m_1+m_2+...+m_r = N-m_{r+1}} \\frac{N!}{m_1!m_2!...m_r!m_{r+1}!} \\prod_{k=1}^{r+1} x_k^{m_k} \\right)$\n",
    "\n",
    "Note: $\\sum_{m_{r+1}=0}^N \\left(\\sum_{m_1+m_2+...+m_r = N-m_{r+1}} (\\cdot) \\right) = \\sum_{m_1+m_2+...+m_r+m_{r+1} = N} (\\cdot)$\n",
    "\n",
    "$= \\sum_{m_1+m_2+...+m_r+m_{r+1} = N} \\frac{N!}{m_1!m_2!...m_r!m_{r+1}!} \\prod_{k=1}^{r+1} x_k^{m_k}$\n",
    "\n",
    "#### References \n",
    "\n",
    "[proofwiki.org - Multinomial Theorem](https://proofwiki.org/wiki/Multinomial_Theorem)"
   ]
  }
 ],
 "metadata": {
  "kernelspec": {
   "display_name": "Python 3",
   "language": "python",
   "name": "python3"
  },
  "language_info": {
   "codemirror_mode": {
    "name": "ipython",
    "version": 3
   },
   "file_extension": ".py",
   "mimetype": "text/x-python",
   "name": "python",
   "nbconvert_exporter": "python",
   "pygments_lexer": "ipython3",
   "version": "3.5.6"
  }
 },
 "nbformat": 4,
 "nbformat_minor": 2
}
