{
 "cells": [
  {
   "cell_type": "markdown",
   "metadata": {},
   "source": [
    "# Gamma function and Beta function\n",
    "\n",
    "[Back to index](https://shotahorii.github.io/math-for-ds/)\n",
    "\n",
    "---\n",
    "\n",
    "## Table of contents\n",
    "1. **Gamma function**  \n",
    "1.1. Definition  \n",
    "1.2. When $z$ is a natural number\n",
    "2. **Beta function**  \n",
    "2.1. Definition  \n",
    "2.2. Symmetricity \n",
    "3. **Relationship between Gamma function and Beta function**  \n",
    "3.1. Change of variable for Gamma function  \n",
    "3.2. Change of variable for Beta function  \n",
    "3.3. Relationship equation\n",
    "4. **Multivariate beta function**\n",
    "\n",
    "---\n",
    "\n",
    "## 1. Gamma function\n",
    "### 1.1. Definition\n",
    "For complex numbers with a positive real part $z$,\n",
    "\n",
    "$ \\Gamma(z) = \\int^\\infty_0 \\mu^{z-1}e^{-\\mu}d\\mu$\n",
    "\n",
    "$where \\,\\,\\,\\, Re(z) > 0 $\n",
    "\n",
    "Also below equation is true. \n",
    "\n",
    "$ \\Gamma(z+1) = z\\Gamma(z) $\n",
    "\n",
    "**Proof**\n",
    "\n",
    "$ \\Gamma(z+1) =  \\int^\\infty_0 \\mu^z e^{-\\mu}d\\mu$\n",
    "\n",
    "$ = \\int^\\infty_0 \\mu^z (-e^{-\\mu})'d\\mu $\n",
    "\n",
    "Using integration by parts,\n",
    "\n",
    "$ = [-\\mu^z e^{-\\mu}]^\\infty_0 + \\int^\\infty_0 z\\mu^{z-1} e^{-\\mu}d\\mu $\n",
    "\n",
    "$ = \\lim\\limits_{\\mu \\to \\infty}(-\\mu^ze^{-\\mu}) - (-0e^{-0}) + \\int^\\infty_0 z\\mu^{z-1} e^{-\\mu}d\\mu $\n",
    "\n",
    "Note: $ \\lim\\limits_{x \\to \\infty}(-x^ze^{-x}) = 0 $\n",
    "\n",
    "$ = \\int^\\infty_0 z\\mu^{z-1} e^{-\\mu}d\\mu $\n",
    "\n",
    "$ = z\\int^\\infty_0 \\mu^{z-1} e^{-\\mu}d\\mu = z\\Gamma(z)$\n",
    "\n",
    "---\n",
    "\n",
    "### 1.2. When $z$ is a natural number\n",
    "\n",
    "$ \\Gamma(n) = (n-1)! $\n",
    "\n",
    "$ where\\,\\,\\,\\, n \\in \\mathbb{N} $\n",
    "\n",
    "**Proof**\n",
    "\n",
    "$ \\Gamma(1) = \\int^\\infty_0 \\mu^{1-1}e^{-\\mu}d\\mu = \\int^\\infty_0 e^{-\\mu}d\\mu$\n",
    "\n",
    "$ = \\lim\\limits_{\\mu \\to \\infty}(-e^{-\\mu}) - (-e^{-0}) = 0 - (-1) = 1$\n",
    "\n",
    "Given that $ \\Gamma(1) = 1 $ and $ \\Gamma(z+1) = z\\Gamma(z) $,\n",
    "\n",
    "$ \\Gamma(n) = 1\\cdot2\\cdot3\\cdot\\cdot\\cdot(n-1) = (n-1)!$\n",
    "\n",
    "---\n",
    "\n",
    "## 2. Beta function\n",
    "### 2.1. Definition\n",
    "For complex numbers with a positive real part $a,b$,\n",
    "\n",
    "$ B(a,b) = \\int^1_0 \\mu^{a-1}(1-\\mu)^{b-1}d\\mu$\n",
    "\n",
    "$where \\,\\,\\,\\, Re(a) > 0 \\,\\,\\,\\, Re(b) > 0$\n",
    "\n",
    "---\n",
    "\n",
    "### 2.2. Symmetricity\n",
    "\n",
    "$B(a,b) = B(b,a)$\n",
    "\n",
    "**Proof**\n",
    "\n",
    "$B(a,b) = \\int^1_0 \\mu^{a-1}(1-\\mu)^{b-1}d\\mu$\n",
    "\n",
    "Let: $ \\mu' = 1-\\mu$\n",
    "\n",
    "$ = \\int^1_0 (1-\\mu')^{a-1}(\\mu')^{b-1}d\\mu' = B(b,a)$\n",
    "\n",
    "---\n",
    "\n",
    "## 3. Relationship between Gamma function and Beta function\n",
    "### 3.1. Change of variable for Gamma function\n",
    "\n",
    "$ \\Gamma(z) = \\int^\\infty_0 \\mu^{z-1}e^{-\\mu}d\\mu$\n",
    "\n",
    "Change the variable $\\mu$ as below.\n",
    "\n",
    "$\\mu = r^2 \\,\\,\\, where \\,\\,\\, r \\ge 0$\n",
    "\n",
    "Interval doesn't change. $\\mu \\in [0,\\infty] \\Longrightarrow r^2 \\in [0,\\infty]$\n",
    "\n",
    "Note: $\\int^b_a f(x)dx = \\int^\\beta_\\alpha f(g(t))\\frac{dx}{dt}dt = \\int^\\beta_\\alpha f(g(t))g'(t)dt \\,\\,\\, where \\,\\,\\, g(\\alpha)=a, g(\\beta)=b$\n",
    "\n",
    "$ \\Gamma(z) = \\int^\\infty_0 (r^2)^{z-1}e^{-r^2}\\frac{d}{dr}(r^2)dr \n",
    "= 2\\int^\\infty_0 r^{2z-2}e^{-r^2}rdr = 2\\int^\\infty_0 r^{2z-1}e^{-r^2}dr$\n",
    "\n",
    "---\n",
    "\n",
    "### 3.2. Change of variable for Beta function\n",
    "\n",
    "$B(a,b) = \\int^1_0 \\mu^{a-1}(1-\\mu)^{b-1}d\\mu$\n",
    "\n",
    "Change the variable $\\mu$ as below.\n",
    "\n",
    "$\\mu = sin^2\\theta$\n",
    "\n",
    "Interval changes as $\\mu \\in [0,1] \\Longrightarrow \\theta \\in [0,\\frac{\\pi}{2}]$\n",
    "\n",
    "$B(a,b) = \\int^{\\frac{\\pi}{2}}_0 (sin^2\\theta)^{a-1}(1-sin^2\\theta)^{b-1}\\frac{d}{d\\theta}(sin^2\\theta)d\\theta$\n",
    "\n",
    "$=\\int^{\\frac{\\pi}{2}}_0 (sin^2\\theta)^{a-1}(cos^2\\theta)^{b-1}2sin\\theta cos\\theta d\\theta$\n",
    "\n",
    "$=\\int^{\\frac{\\pi}{2}}_0 sin^{2a-2}\\theta \\, cos^{2b-2}\\theta \\, 2sin\\theta cos\\theta d\\theta$\n",
    "\n",
    "$=2\\int^{\\frac{\\pi}{2}}_0 sin^{2a-1}\\theta \\, cos^{2b-1}\\theta \\, d\\theta$\n",
    "\n",
    "---\n",
    "\n",
    "### 3.3. Relationship equation\n",
    "\n",
    "$\\Gamma(a)\\Gamma(b) = 2\\int^\\infty_0 u^{2a-1}e^{-u^2}du \\cdot 2\\int^\\infty_0 v^{2b-1}e^{-v^2}dv$\n",
    "\n",
    "$= 4\\int^\\infty_0\\int^\\infty_0 e^{-(u^2+v^2)} u^{2a-1} v^{2b-1} dudv$\n",
    "\n",
    "Change the variables $u,v$ as below. (Polar conversion)\n",
    "\n",
    "$u=rcos\\theta, \\,\\,\\, v = rsin\\theta$\n",
    "\n",
    "Interval changes as $u \\in [0,\\infty], \\,\\, v \\in [0,\\infty] \\Longrightarrow r \\in [0,\\infty], \\,\\, \\theta \\in [0,\\frac{\\pi}{2}]$\n",
    "\n",
    "Note: $dudv = rdrd\\theta$ because $det(J_{(r,\\theta)})=r$. Please see Jacobian.\n",
    "\n",
    "$= 4\\int^{\\frac{\\pi}{2}}_0\\int^\\infty_0 e^{-(r^2cos^2\\theta+r^2sin^2\\theta)} (rcos\\theta)^{2a-1} (rsin\\theta)^{2b-1} rdrd\\theta$\n",
    "\n",
    "$= 4 \\int^\\infty_0 e^{-r^2} r^{2a-1}r^{2b-1} rdr \\cdot \\int^{\\frac{\\pi}{2}}_0 cos^{2a-1}\\theta sin^{2b-1}\\theta d\\theta$\n",
    "\n",
    "$= 2 \\int^\\infty_0 r^{2(a+b)-1}e^{-r^2}dr \\cdot 2 \\int^{\\frac{\\pi}{2}}_0 cos^{2a-1}\\theta sin^{2b-1}\\theta d\\theta$\n",
    "\n",
    "$=\\Gamma(a+b)B(b,a) = \\Gamma(a+b)B(a,b)$\n",
    "\n",
    "Hence,\n",
    "\n",
    "$B(a,b) = \\frac{\\Gamma(a)\\Gamma(b)}{\\Gamma(a+b)}$\n",
    "\n",
    "Note: Regarding $ \\int A \\int B = \\int\\int AB $ part, see Fubini's theorem.\n",
    "\n",
    "---\n",
    "\n",
    "## 4. Multivariate beta function\n",
    "\n",
    "$B({\\bf \\alpha}) = \\frac{\\prod_{k=1}^K\\Gamma(\\alpha_k)}{\\Gamma(\\sum_{k=1}^K \\alpha_k)}$\n",
    "\n",
    "$where \\,\\,\\, {\\bf \\alpha} = (\\alpha_1,\\alpha_2,...,\\alpha_K)^T$"
   ]
  }
 ],
 "metadata": {
  "kernelspec": {
   "display_name": "Python 3",
   "language": "python",
   "name": "python3"
  },
  "language_info": {
   "codemirror_mode": {
    "name": "ipython",
    "version": 3
   },
   "file_extension": ".py",
   "mimetype": "text/x-python",
   "name": "python",
   "nbconvert_exporter": "python",
   "pygments_lexer": "ipython3",
   "version": "3.5.6"
  }
 },
 "nbformat": 4,
 "nbformat_minor": 2
}
