{
 "cells": [
  {
   "cell_type": "markdown",
   "metadata": {},
   "source": [
    "# Product Rule\n",
    "\n",
    "[Back to index](https://shotahorii.github.io/math-for-ds/)\n",
    "\n",
    "---\n",
    "\n",
    "## Table of contents\n",
    "1. Product Rule\n",
    "2. General Leibniz rule\n",
    "3. More than two factors\n",
    "\n",
    "---"
   ]
  },
  {
   "cell_type": "markdown",
   "metadata": {},
   "source": [
    "## 1. Product Rule\n",
    "\n",
    "$(f\\cdot g)' = f'\\cdot g + f \\cdot g'$\n",
    "\n",
    "**Proof1**\n",
    "\n",
    "Let: $h(x) = f(x)g(x)$\n",
    "\n",
    "$h'(x) = \\lim\\limits_{\\Delta x \\to 0}\\frac{h(x+\\Delta x)-h(x)}{\\Delta x}$\n",
    "\n",
    "$= \\lim\\limits_{\\Delta x \\to 0}\\frac{f(x+\\Delta x)g(x+\\Delta x)-f(x)g(x)}{\\Delta x}$\n",
    "\n",
    "$= \\lim\\limits_{\\Delta x \\to 0}\\frac{f(x+\\Delta x)g(x+\\Delta x) - f(x)g(x+\\Delta x) + f(x)g(x+\\Delta x) -f(x)g(x)}{\\Delta x}$\n",
    "\n",
    "$= \\lim\\limits_{\\Delta x \\to 0}\\frac{\\{f(x+\\Delta x)-f(x)\\}g(x+\\Delta x) + f(x)\\{g(x+\\Delta x) - g(x)\\}}{\\Delta x}$\n",
    "\n",
    "$= \\lim\\limits_{\\Delta x \\to 0}\\frac{f(x+\\Delta x)-f(x)}{\\Delta x} \\lim\\limits_{\\Delta x \\to 0}g(x+\\Delta x)\n",
    "+ \\lim\\limits_{\\Delta x \\to 0}f(x) \\lim\\limits_{\\Delta x \\to 0}\\frac{g(x+\\Delta x)-g(x)}{\\Delta x}$\n",
    "\n",
    "$=f'(x)g(x) + f(x)g'(x)$\n",
    "\n",
    "Note: The fact that $\\lim\\limits_{\\Delta x \\to 0}g(x+\\Delta x) = g(x)$ is deduced from a theorem that states that differentiable functions are continuous.\n",
    "\n",
    "**Proof2**\n",
    "\n",
    "Let: $h(u,v) = uv, \\,\\, u = f(x), \\,\\, v = g(x)$\n",
    "\n",
    "With the chain rule,\n",
    "\n",
    "$\\frac{dh}{dx} = \\frac{dh}{du}\\frac{du}{dx} + \\frac{dh}{dv}\\frac{dv}{dx}$\n",
    "\n",
    "$= v \\cdot f'(x) + u \\cdot g'(x)$\n",
    "\n",
    "$= g(x)f'(x) + f(x)g'(x)$\n",
    "\n",
    "---"
   ]
  },
  {
   "cell_type": "markdown",
   "metadata": {},
   "source": [
    "## 2. General Leibniz rule\n",
    "\n",
    "$(fg)^{(n)} = \\sum_{k=0}^n \\left(\\begin{array}{c}n\\\\k\\\\\\end{array}\\right) f^{(n-k)}g^{(k)}$\n",
    "\n",
    "**Proof**\n",
    "\n",
    "The proof of the general Leibniz rule proceeds by induction. Let $f$ and $g$ be $n$-times differentiable functions.  \n",
    "When $n=1$, the general Leibniz rule is true because of the usual product rule, as below.\n",
    "\n",
    "$(fg)^{(1)} = \\sum_{k=0}^1 \\left(\\begin{array}{c}1\\\\k\\\\\\end{array}\\right) f^{(1-k)}g^{(k)}\n",
    "= \\left(\\begin{array}{c}1\\\\0\\\\\\end{array}\\right) f^{(1)}g^{(0)} + \\left(\\begin{array}{c}1\\\\1\\\\\\end{array}\\right) f^{(0)}g^{(1)} = f'g+fg'\n",
    "$\n",
    "\n",
    "Now, assume the general Leibniz rule is true when $n=N$, \n",
    "\n",
    "$(fg)^{(N)} = \\sum_{k=0}^N \\left(\\begin{array}{c}N\\\\k\\\\\\end{array}\\right) f^{(N-k)}g^{(k)}$\n",
    "\n",
    "Then,\n",
    "\n",
    "$(fg)^{(N+1)} = \\{\\sum_{k=0}^N \\left(\\begin{array}{c}N\\\\k\\\\\\end{array}\\right) f^{(N-k)}g^{(k)}\\}'$\n",
    "\n",
    "Considering the linearity of differentiation,\n",
    "\n",
    "$=\\sum_{k=0}^N \\left(\\begin{array}{c}N\\\\k\\\\\\end{array}\\right) \\{f^{(N-k)}g^{(k)}\\}'$\n",
    "\n",
    "$=\\sum_{k=0}^N \\left(\\begin{array}{c}N\\\\k\\\\\\end{array}\\right) \\{f^{(N-k+1)}g^{(k)} + f^{(N-k)}g^{(k+1)}\\}$\n",
    "\n",
    "$=\\sum_{k=0}^N \\left(\\begin{array}{c}N\\\\k\\\\\\end{array}\\right) f^{(N-k+1)}g^{(k)} + \\sum_{k=0}^N \\left(\\begin{array}{c}N\\\\k\\\\\\end{array}\\right) f^{(N-k)}g^{(k+1)}$\n",
    "\n",
    "Shift the second term from $\\sum_{k=0}^N$ to $\\sum_{k=1}^{N+1}$\n",
    "\n",
    "$=\\sum_{k=0}^N \\left(\\begin{array}{c}N\\\\k\\\\\\end{array}\\right) f^{(N-k+1)}g^{(k)} + \\sum_{k=1}^{N+1} \\left(\\begin{array}{c}N\\\\k-1\\\\\\end{array}\\right) f^{(N-k+1)}g^{(k)}$\n",
    "\n",
    "$=\\left(\\begin{array}{c}N\\\\0\\\\\\end{array}\\right) f^{(N+1)}g^{(0)} + \\sum_{k=1}^N \\left(\\begin{array}{c}N\\\\k\\\\\\end{array}\\right) f^{(N-k+1)}g^{(k)} + \\sum_{k=1}^{N} \\left(\\begin{array}{c}N\\\\k-1\\\\\\end{array}\\right) f^{(N-k+1)}g^{(k)} + \\left(\\begin{array}{c}N\\\\N\\\\\\end{array}\\right) f^{(0)}g^{(N+1)}$\n",
    "\n",
    "$=f^{(N+1)}g^{(0)} + \\sum_{k=1}^N \\{\\left(\\begin{array}{c}N\\\\k\\\\\\end{array}\\right)+\\left(\\begin{array}{c}N\\\\k-1\\\\\\end{array}\\right)\\} f^{(N-k+1)}g^{(k)} + f^{(0)}g^{(N+1)}$\n",
    "\n",
    "Using the [property of binomial coefficient](https://github.com/shotahorii/math-for-ds/blob/master/content/others/binomial_coefficient.ipynb),\n",
    "\n",
    "$=f^{(N+1)}g^{(0)} + \\sum_{k=1}^N \\left(\\begin{array}{c}N+1\\\\k\\\\\\end{array}\\right) f^{(N-k+1)}g^{(k)} + f^{(0)}g^{(N+1)}$\n",
    "\n",
    "$=\\sum_{k=0}^{N+1} \\left(\\begin{array}{c}N+1\\\\k\\\\\\end{array}\\right) f^{(N-k+1)}g^{(k)}$\n",
    "\n",
    "Now proof is complete as the rule is true for $n=N+1$ when it's true for $n=N$\n",
    "\n",
    "---"
   ]
  },
  {
   "cell_type": "markdown",
   "metadata": {},
   "source": [
    "## 3. More than two factors\n",
    "\n",
    "$$(f_1f_2...f_m)^{(n)} = \\sum_{k_i \\in \\mathbb{N}_0, \\sum_{i=1}^m k_i = n} \\left(\\frac{n!}{\\prod_{i=1}^mk_i!}\\prod_{i=1}^mf_i^{(k_i)}\\right)$$\n",
    "\n",
    "where the sum extends over all m-tuples $(k_1,...,k_m)$ of non-negative integers with $\\sum_{i=1}^mk_i! = n$\n",
    "\n",
    "**Example**\n",
    "\n",
    "Let: $n=1$, $m=3$ then,\n",
    "\n",
    "$(f_1f_2f_3)' = \\sum_{k_i \\in \\mathbb{N}_0, \\sum_{i=1}^3 k_i = 1} \\left(\\frac{1!}{\\prod_{i=1}^3k_i!}\\prod_{i=1}^3f_i^{(k_i)}\\right)$\n",
    "\n",
    "Note: the sum here extends over $(k_1=1,k_2=0,k_3=0)$, $(k_1=0,k_2=1,k_3=0)$ and $(k_1=0,k_2=0,k_3=1)$\n",
    "\n",
    "$= \\left(\\frac{1!}{1!0!0!}f_1^{(1)}f_2^{(0)}f_3^{(0)} \\right) + \\left(\\frac{1!}{0!1!0!}f_1^{(0)}f_2^{(1)}f_3^{(0)} \\right) + \\left(\\frac{1!}{0!0!1!}f_1^{(0)}f_2^{(0)}f_3^{(1)} \\right)$\n",
    "\n",
    "$= f_1'f_2f_3 + f_1f_2'f_3 + f_1f_2f_3'$"
   ]
  }
 ],
 "metadata": {
  "kernelspec": {
   "display_name": "Python 3",
   "language": "python",
   "name": "python3"
  },
  "language_info": {
   "codemirror_mode": {
    "name": "ipython",
    "version": 3
   },
   "file_extension": ".py",
   "mimetype": "text/x-python",
   "name": "python",
   "nbconvert_exporter": "python",
   "pygments_lexer": "ipython3",
   "version": "3.5.6"
  }
 },
 "nbformat": 4,
 "nbformat_minor": 2
}
